theories/examples/malloc.v
@@ -24,22 +24,24 @@ Section malloc.
   Global Parameter e_m : Addr.
   Global Parameter a_m : Addr.
 
-  Global Parameter malloc_subroutine : RegName -> nat -> list Word.
+  Global Parameter malloc_subroutine : list Word.
+  Global Parameter malloc_γ : namespace. 
   
-  Global Axiom malloc_spec : forall (W : WORLD) (size : nat) (continuation : Word) (r : RegName) φ, 
+  Global Axiom malloc_subroutine_spec : forall (W : WORLD) (size : Z) (continuation : Word) wsr φ, 
   ( (* the malloc subroutine and parameters *)
-       [[b_m,e_m]] ↦ₐ[p_m] [[malloc_subroutine r size]]
+       inv malloc_γ ([[b_m,e_m]] ↦ₐ[p_m] [[malloc_subroutine]])
      ∗ r_t0 ↦ᵣ continuation
      (* the PC points to the malloc subroutine *)
      ∗ PC ↦ᵣ inr (RX,Global,b_m,e_m,a_m)
+     ∗ r_t1 ↦ᵣ inl size
     (* we pass control of all general purpose registers *)
-     ∗ (∃ wsr, [∗ list] r_i;w_i ∈ list_difference all_registers [PC;r_t0]; wsr, r_i ↦ᵣ w_i)
+     ∗ ([∗ list] r_i;w_i ∈ list_difference all_registers [PC;r_t0;r_t1]; wsr, r_i ↦ᵣ w_i)
     (* continuation *)
-     ∗ ▷ (([[b_m,e_m]] ↦ₐ[p_m] [[malloc_subroutine r size]]
-        ∗ (∃ wsr, [∗ list] r_i;w_i ∈ list_difference all_registers [PC;r]; wsr, r_i ↦ᵣ w_i)
+     ∗ ▷ ((([∗ list] r_i;w_i ∈ list_difference all_registers [PC;r_t0;r_t1]; wsr, r_i ↦ᵣ w_i)
+        ∗ r_t0 ↦ᵣ continuation                                                                                     
         ∗ PC ↦ᵣ continuation
         (* the newly allocated region *)
-        ∗ ∃ (b e : Addr), ⌜(e - b = size - 1)%Z⌝ ∧ r ↦ᵣ inr (RWX,Global,b,e,b)
+        ∗ ∃ (b e : Addr), ⌜(e - b = size)%Z⌝ ∧ r_t1 ↦ᵣ inr (RWX,Global,b,e,b)
         ∗ [[b,e]] ↦ₐ[RWX] [[region_addrs_zeroes b e]]
         (* the allocated region is guaranteed to be fresh in the provided world *)
         (* TODO: remove this is we can prove it *)
@@ -47,6 +49,6 @@ Section malloc.
                       ∧ (countable.encode a) ∉ dom (gset positive) (std_rel W)) (region_addrs b e)⌝)
         -∗ WP Seq (Instr Executable) {{ φ }})
      ⊢ WP Seq (Instr Executable) {{ φ }})%I.
-
+  
 End malloc.   
   
